Zip/Spec/LZ77L5Correct.lean
@@ -245,7 +245,7 @@ theorem lz77ChainLazyIterPMergedL5Large_eq (data : ByteArray)
       · dsimp only
         exact noH3SingleLoop_eq data windowSize 65536
           (min chainWinSize data.size) 22 insertCap goodMatch niceLen 5 1
-          (by omega) _ (Array.replicate 32768 data.size) 0 _
+          (by omega) _ (initialH3Table false data.size) 0 _
     _ = lz77ChainLazyIterP data 22 windowSize insertCap goodMatch niceLen
           5 false 1 :=
       lz77ChainLazyIterPMerged_eq data 22 windowSize insertCap goodMatch niceLen
